\begin{aligned}
&A = \begin{bmatrix}
1 & -2 &  6 \\
4 &  3 & -8 \\
2 & -2 &  5
\end{bmatrix} \\
&3A + 2X = I_{3} \\

& \iff X = \frac{(I_{3} - 3A)}{2} \\
& \iff X = \frac{1}{2}
\Bigg( \begin{bmatrix}
	1 & 0 & 0 \\
	0 & 1 & 0 \\
	0 & 0 & 1
	\end{bmatrix}
	- 3 \begin{bmatrix}
	1 & -2 &  6 \\
	4 &  3 & -8 \\
	2 & -2 &  5
	\end{bmatrix}
\Bigg ) \\

& \iff X = \frac{1}{2}
\begin{bmatrix}
-2 & 6 & -18 \\
-12 & -8 & 24 \\
-6 & 6 & -14
\end{bmatrix} \\

& \iff X = \begin{bmatrix}
-1 & 3 & -9 \\
-6 & -4 & 12 \\
-3 & 3 & -7
\end{bmatrix} \\
\end{aligned}
