\begin{aligned}
&\text{a)} \begin{vmatrix}
1 & 1 & 1 \\
-1 & 0 & 1 \\
-1 & -1 & 0
\end{vmatrix}
\begin{matrix}
1 & 1 \\
-1 & 0 \\
-1 & -1
\end{matrix} \\
&= 1.0.0 + 1.1.(-1) + 1.(-1).(-1) - (-1).0.1 - (-1).1.1 - 0.(-1).1 \\
&= -1 + 1 + 1 = 1 \\
\\



&\text{b)} \begin{vmatrix}
0 & 1 & 1 \\
1 & 0 & 1 \\
1 & 1 & 0
\end{vmatrix}
\begin{matrix}
0 & 1 \\
1 & 0 \\
1 & 1 
\end{matrix} \\
&=0.0.0 + 1.1.1 + 1.1.1 - 1.0.1 - 1.1.0 - 0.1.1 \\
&=2 \\
\\


&\text{c)} \begin{vmatrix}
2 & 1  & 1 \\
0 & 5  & -2 \\
1 & -3 & 4 \\
\end{vmatrix}
\begin{matrix}
2 & 1  \\
0 & 5  \\
1 & -3 \\
\end{matrix} \\
&= 2.5.4 + 1.(-2).1 + 1.0.(-3) - 1.5.1 - (-3).(-2).2 - 4.0.1 \\
&= 40 -2 -5 -12 = 21 \\
\\


&\text{d)} \begin{vmatrix}
3 & -2 & -4 \\
2 & 5 & -1 \\
0 & 6 & 1 \\
\end{vmatrix}
\begin{matrix}
3 & -2 \\
2 & 5 \\
0 & 6 \\
\end{matrix} \\
&=3.5.1 +(-2).(-1).0 + (-4).2.6 - 0.5.(-4) - 6.(-1).3 - 1.2.(-2) \\
&=15 - 48 - 18 +4 = 47 \\
\\


&\text{e)} \begin{vmatrix}
-2 & -1 &  4 \\
 6 & -3 & -2 \\
 4 &  1 &  2 \\
\end{vmatrix}
\begin{matrix}
-2 & -1 \\
 6 & -3 \\
 4 &  1 \\
\end{matrix} \\
&=(-2).(-3).2 + (-1).(-2).4 +  4.6.1 - 4.(-3).4 - 1.(-2).(-2) - 2.6.(-1) \\
&= 12 + 8 + 24 + 48 - 4 + 12 = 88 \\
\\



&\text{f)} \begin{vmatrix}
7 & 6 & 5 \\
1 & 2 & 1 \\
3 & -2 & 1 \\
\end{vmatrix}
\begin{matrix}
7 & 6 \\
1 & 2 \\
3 & -2 \\
\end{matrix} \\
&= 7.2.1 + 6.1.3 + 5.1.(-2) - 3.2.5 +(-2).1.7 - 1.1.6 \\
&= 14 +18 -10 -30 -14 -6 \\
&=-28 \\
\\

&\text{g)} \begin{vmatrix}
1 & 2  & 3 \\
4 & -2 & 3 \\
0 & 5  & -1 \\
\end{vmatrix}
\begin{matrix}
1 & 2  \\
4 & -2 \\
0 & 5  \\
\end{matrix} \\
&=1.(-2).(-1) + 2.3.0 + 3.4.5 - 0.(-2).3 -5.3.1 - (-1).4.2 \\
&= 2 + 60 -15 +8 = 55 \\
\\


&\text{h)}
\begin{vmatrix}
2 & 3 & 4 \\
5 & 6 & 7 \\
8 & 9 & 1 \\
\end{vmatrix}
\begin{matrix}
2 & 3  \\
5 & 6  \\
8 & 9  \\
\end{matrix} \\
&= 2.6.1+3.7.8+4.5.9-8.6.4-9.7.2-1.5.3 \\
&= 27 \\
\\

&\text{i)}
\begin{vmatrix}
2 & 0 & 1 \\
3 & 2 & -3 \\
-1 & -3 & 5 \\
\end{vmatrix}
\begin{matrix}
2 & 0  \\
3 & 2   \\
-1 & -3 \\
\end{matrix} \\
&= 2.2.5 + 0.(-3).(-1) -(-1).2.1 - (-3).(-3).2 - 5.3.0  \\
&= 4 \\
\\


&\text{j)}
\begin{vmatrix}
1 & 0 & 0 \\
3 & 2 & -4 \\
4 & 1 & 3 \\
\end{vmatrix}
\begin{matrix}
1 & 0 \\
3 & 2 \\
4 & 1 \\
\end{matrix} \\
&=1.2.3 + 0.(-4).4 +0.3.1 -4.2.0 - 1.(-4).1 -3.3.0 \\
&=10 \\
\\







\end{aligned}
