\begin{aligned}

&\begin{vmatrix}
x & 1 & 1 & 1 \\
1 & x & 1 & 1 \\
1 & 1 & x & 1 \\
1 & 1 & 1 & x \\
\end{vmatrix} \\

&= -\begin{vmatrix}
1 & 1 & 1 & x \\
1 & x & 1 & 1 \\
1 & 1 & x & 1 \\
x & 1 & 1 & 1 \\
\end{vmatrix} \begin{bmatrix}(1) \sim (4)\end{bmatrix} \\



&= -\begin{vmatrix}
1 & 1 & 1 & x \\
0 & x-1 & 0 & 1-x \\
0 & 0 & x-1 & 1-x \\
0 & 1-x & 1-x & 1-x^2 \\
\end{vmatrix}
\begin{bmatrix}
(2):=(2) - (1) \\
(3):=(3) - (1) \\
(4):=(4) - x(1) \\
\end{bmatrix} \\


&= -\begin{vmatrix}
1 & 1 & 1 & x \\
0 & x-1 & 0 & 1-x \\
0 & 0 & x-1 & 1-x \\
0 & 0 & 1-x & (1-x)(x+2) \\
\end{vmatrix}
\begin{bmatrix}
(4):=(4) + (2) \\
\end{bmatrix} \\


&= -\begin{vmatrix}
1 & 1 & 1 & x \\
0 & x-1 & 0 & 1-x \\
0 & 0 & x-1 & 1-x \\
0 & 0 & 0 & (1-x)(x+3) \\
\end{vmatrix}
\begin{bmatrix}
(4):=(4) + (3) \\
\end{bmatrix} \\
&=-(x-1)^2(1-x)(x+3) = (x-1)^3(x+3) \\
\\

\end{aligned} 
