\begin{aligned}
&\begin{vmatrix}
1 & 1 & 1 & 0 \\
1 & 1 & 0 & 1 \\
1 & 0 & 1 & 1 \\
0 & 1 & 1 & 1 \\
\end{vmatrix} \\
&=\begin{vmatrix}
1 & 1 & 1 & 0 \\
0 & 0 & -1 & 1 \\
0 & -1 & 0 & 1 \\
0 & 1 & 1 & 1 \\
\end{vmatrix} \begin{bmatrix}
	(2):=(2)-(1) \\
	(3):=(3)-(1) \\
\end{bmatrix} \\


&=-\begin{vmatrix}
1 & 1 & 1 & 0 \\
0 & 1 & 1 & 1 \\
0 & -1 & 0 & 1 \\
0 & 0 & -1 & 1 \\
\end{vmatrix} \begin{bmatrix}
	(2) \sim (4) \\
\end{bmatrix} \\


&=-\begin{vmatrix}
1 & 1 & 1 & 0 \\
0 & 1 & 1 & 1 \\
0 & 0 & 1 & 2 \\
0 & 0 & -1 & 1 \\
\end{vmatrix} \begin{bmatrix}
	(3):=(3) + (2)
\end{bmatrix} \\


&=-\begin{vmatrix}
1 & 1 & 1 & 0 \\
0 & 1 & 1 & 1 \\
0 & 0 & 1 & 2 \\
0 & 0 & 0 & 3 \\
\end{vmatrix} \begin{bmatrix}
	(4):=(4) + (3)
\end{bmatrix} \\
&=-3 \\
\\
\end{aligned} \\
