\begin{aligned}
A&=\begin{bmatrix}
2 & 5 & -1 \\
3 & 0  & -4
\end{bmatrix}
; B = \begin{bmatrix}
1 & -2 & -3 \\
0 & -1 & 5
\end{bmatrix}
; C = \begin{bmatrix}
0 & 1 & -2 \\
1 & -1 & -1
\end{bmatrix} \\
3A + 4B - 2C
&= 3\begin{bmatrix}
2 & 5 & -1 \\
3 & 0  & -4
\end{bmatrix}
+4 \begin{bmatrix}
1 & -2 & -3 \\
0 & -1 & 5
\end{bmatrix}
-2 \begin{bmatrix}
0 & 1 & -2 \\
1 & -1 & -1
\end{bmatrix} \\
&= 
\begin{bmatrix}
6 & 15 & -3 \\
9 & 0  & -12
\end{bmatrix}
+ \begin{bmatrix}
4 & -8 & -12 \\
0 & -4 & 20
\end{bmatrix}
-\begin{bmatrix}
0 & 2 & -4 \\
2 & -2 & -2
\end{bmatrix} \\
&=\begin{bmatrix}
6 + 4 - 0 & 15 -8 - 2 & -3 -12 + 4 \\
9 + 0 - 2 & 0 - 4 + 2 & -12 + 20 + 2
\end{bmatrix} \\
&=\begin{bmatrix}
10 & 5 & -11 \\
7 & -2 & 10
\end{bmatrix}
\end{aligned}
