\begin{aligned}

A&=\begin{bmatrix}
2 & 1 & -1 \\
0 & 1 & -4
\end{bmatrix};
B=\begin{bmatrix}
 2 & 1 & 0 \\
-3 & 2 & 2
\end{bmatrix} \\
\\

3A + 2B &=3\begin{bmatrix}
2 & 1 & -1 \\
0 & 1 & -4
\end{bmatrix}
+2\begin{bmatrix}
 2 & 1 & 0 \\
-3 & 2 & 2
\end{bmatrix} \\

&=\begin{bmatrix}
6+4 & 3+2 & -3 + 0 \\
0-6 & 3+4 & -12 + 4
\end{bmatrix} \\

&=\begin{bmatrix}
10 & 5 & -3 \\
-6 & 7 & -8
\end{bmatrix};

\\
3A - 2B &=3\begin{bmatrix}
2 & 1 & -1 \\
0 & 1 & -4
\end{bmatrix}
-2\begin{bmatrix}
 2 & 1 & 0 \\
-3 & 2 & 2
\end{bmatrix} \\

&=\begin{bmatrix}
6-4 & 3-2 & -3 - 0 \\
0+6 & 3-4 & -12 - 4
\end{bmatrix} \\

&=\begin{bmatrix}
2 & 1  & -3 \\
6 & -1 & -16
\end{bmatrix}; \\

\\

A^{T}A&=\begin{bmatrix}
2  & 0 \\
1  & 1 \\
-1 & -4
\end{bmatrix}
\begin{bmatrix}
2 & 1 & -1 \\
0 & 1 & -4
\end{bmatrix} \\

&=\begin{bmatrix}
2 . 2 + 0.0 & 2 .1 + 0.1 & 2 (-1) + 0(-4) \\
1 . 2 + 1.0 & 1 .1 + 1.1 & 1 (-1) + 1(-4) \\
-1. 2 - 4.0 & -1.1 - 4.1 & -1(-1) - 4(-4)
\end{bmatrix} \\

&=\begin{bmatrix}
4 & 2 & -2 \\
2 & 2 & -5 \\
-2 & -5 & 17
\end{bmatrix}; \\

AA^{T}&=\begin{bmatrix}
2 & 1 & -1 \\
0 & 1 & -4
\end{bmatrix}
\begin{bmatrix}
2  & 0 \\
1  & 1 \\
-1 & -4
\end{bmatrix} \\

&=\begin{bmatrix}
2.2 + 1.1 - 1(-1) & 2.0 + 1.1 - 1(-4) \\
0.2 + 1.1 - 4(-1) & 0.0 + 1.1 - 4(-4)
\end{bmatrix} \\

&=\begin{bmatrix}
6 & 5 \\
5 & 17
\end{bmatrix} \\

\end{aligned}
