\begin{aligned}
&\text{a) }A = \overline{p} \lor (\overline{q} \rarr p) \\
&\begin{array}{|c |c |c |c |c |c | c |}
p & q & \overline{p} & \overline{q} & \overline{q} \rarr p & A \\
\hline
 1 & 1  & 0  & 0  & 1  & 1  \\
 1 & 0  & 0  & 1  & 1  & 1  \\
 0 & 1  & 1  & 0  & 1  & 1  \\
 0 & 0  & 1  & 1  & 0  & 1  \\
\end{array} \\
\\



&\text{b) } B = r \land ( \overline{q} \lor p) \\
&\begin{array}{| c | c | c | c | c | c |}
p & q & r & \overline{q} & \overline{q} \lor p & B \\
\hline
1 & 1 & 1 & 0 & 1 & 1 \\
1 & 1 & 0 & 0 & 1 & 0 \\
1 & 0 & 1 & 1 & 1 & 1 \\
1 & 0 & 0 & 1 & 1 & 0 \\
0 & 1 & 1 & 0 & 0 & 0 \\
0 & 1 & 0 & 0 & 0 & 0 \\
0 & 0 & 1 & 1 & 1 & 1 \\
0 & 0 & 0 & 1 & 1 & 0 \\
\end{array} \\
\\



&\text{c) } C = (p \land \overline{r}) \rarr \big( q \rarr ( \overline{p} \lor r )  \big) \\
&\begin{array}{| c | c | c | c | c | c | c |}
p & q & r & p \land \overline{r} & \overline{p} \land r & q \rarr ( \overline{p} \lor r ) & C \\
\hline
 1 & 1 & 1 & 0 & 1 & 1 & 1 \\
 1 & 1 & 0 & 1 & 0 & 0 & 0 \\
 1 & 0 & 1 & 0 & 1 & 1 & 1 \\
 1 & 0 & 0 & 1 & 0 & 1 & 1 \\
 0 & 1 & 1 & 0 & 1 & 1 & 1 \\
 0 & 1 & 0 & 0 & 1 & 1 & 1 \\
 0 & 0 & 1 & 0 & 1 & 1 & 1 \\
 0 & 0 & 0 & 0 & 1 & 1 & 1 \\
\end{array} \\
\\












































\end{aligned}
