\begin{aligned}
A &= \begin{bmatrix}
1 & -2 & 3 \\
4 & 5 & -6 \\
\end{bmatrix}
;
B = \begin{bmatrix}
3 & 0 & 2 \\
-7 & 1 & 8
\end{bmatrix}
\\
2A - 3B &= 2
\begin{bmatrix}
1 & -2 & 3 \\
4 & 5 & -6 \\
\end{bmatrix} 
-3 
\begin{bmatrix}
3 & 0 & 2 \\
-7 & 1 & 8
\end{bmatrix} \\
&= \begin{bmatrix}
2 & -4 & 6 \\
8 & 10 & -12 \\
\end{bmatrix} 
-\begin{bmatrix}
9 & 0 & 6 \\
-21 & 3 & 24
\end{bmatrix} \\
&= \begin{bmatrix}
2 & -4 & 6 \\
8 & 10 & -12 \\
\end{bmatrix}  \\\
&= \begin{bmatrix}
	2-9 & -4 - 0 & 6 - 6 \\
	8 + 21 & 3 - 10 & 24 - 12
\end{bmatrix} \\\
&= \begin{bmatrix}
	-7 & -4 & 0 \\
	29 & -7 & 12
\end{bmatrix}
\\
\end{aligned}
