\begin{aligned}
A&=\begin{bmatrix}
2 & -1 \\
1 & 0 \\
-3 & 4
\end{bmatrix} ;
B = \begin{bmatrix}
1 & -2 & 5 \\
3 & 4 & 0
\end{bmatrix}
\\

AB&=\begin{bmatrix}
2 & -1 \\
1 & 0 \\
-3 & 4
\end{bmatrix}
\begin{bmatrix}
1 & -2  &5 \\
3 & 4 & 0
\end{bmatrix} \\

&=\begin{bmatrix}
2.1 -1.3 & 2.(-2) -1.4 & 2.5 -1.0 \\
1.1 + 0.3 & 1.(-2) +0.4 & 1.5 + 0.0 \\
-3.1 + 4.3 & -3.(-2) + 4.4 & -3.5 + 4.0
\end{bmatrix} \\

&=\begin{bmatrix}
-1 & -8 & 10 \\
1 & -2 & 5 \\
9 & 22 & -15
\end{bmatrix} \\
\\
BA&=\begin{bmatrix}
1 & -2  &5 \\
3 & 4 & 0
\end{bmatrix}
\begin{bmatrix}
2 & -1 \\
1 & 0 \\
-3 & 4
\end{bmatrix} \\

&=\begin{bmatrix}
1.2 -2.1 + 5.(-3) & 1.(-1) -2.0 + 5.4 \\
3.2 +4.1 + 0.(-3) & 3.(-1) +4.0 + 0.4
\end{bmatrix} \\

&=\begin{bmatrix}
-15 & 19 \\
10 & -3
\end{bmatrix} \\
\end{aligned}
