\begin{aligned}
A&=\begin{bmatrix}
2 & -1 & 3 \\
0 &  1 & 2
\end{bmatrix},
B=\begin{bmatrix}
-2 &  1 \\
0  &  2 \\
1  & -1
\end{bmatrix},
C=\begin{bmatrix}
1 & 1 \\
0 & 1 
\end{bmatrix} \\

a)& AB, BA, CA, BC \\
b)& AB=? ABC=? \\
c)& (AB)^{3}, C^{n} (n \in \mathbb{N}) \\

AB&=\begin{bmatrix}
2 & -1 & 3 \\
0 &  1 & 2
\end{bmatrix}
\begin{bmatrix}
-2 &  1 \\
0  &  2 \\
1  & -1
\end{bmatrix} \\

&=\begin{bmatrix}
2(-2) - 1.0 + 3.1 & 2.1 - 1.2 + 3(-1) \\
0(-2) + 1.0 + 2.1 & 0.1 + 1.2 + 2(-1) 
\end{bmatrix} \\

&=\begin{bmatrix}
-1 & -3 \\
2 & 0
\end{bmatrix} \\
\\


ABC&=\begin{bmatrix}
2 & -1 & 3 \\
0 &  1 & 2
\end{bmatrix}
\begin{bmatrix}
-2 &  1 \\
0  &  2 \\
1  & -1
\end{bmatrix}
\begin{bmatrix}
1 & 1 \\
0 & 1 
\end{bmatrix} \\


&=\begin{bmatrix}
-1 & -3 \\
2 & 0
\end{bmatrix}
\begin{bmatrix}
1 & 1 \\
0 & 1 
\end{bmatrix} \\

&=\begin{bmatrix}
-1.1 - 3.0 & -1.1 - 3.1 \\
2 .1 + 0.0 & 2 .1 + 0.1
\end{bmatrix} \\

&=\begin{bmatrix}
-1 & -4 \\
2 & 2
\end{bmatrix} \\


(AB)^{3} &= \begin{bmatrix}
-1 & -3 \\
 2 &  0
\end{bmatrix}^{3} \\

&=\begin{bmatrix}
(-1)^{3} & (-3)^{3} \\
 2^{3}   &  0^{3}
\end{bmatrix} \\

&=\begin{bmatrix}
-1 & -27 \\
 8 &  0
\end{bmatrix} \\
\\

C^{1} &= C \\
\text{Suppose that } C^{n} & = \begin{bmatrix}
1 & n \\
0 & 1
\end{bmatrix} \\
\text{We have: } \\
C^{n+1} &= C^{n}C = \begin{bmatrix}
1 & n \\
0 & 1
\end{bmatrix} 
\begin{bmatrix}
1 & 1 \\
0 & 1
\end{bmatrix} \\
&=\begin{bmatrix}
1 & n + 1 \\
0 & 1
\end{bmatrix}

\end{aligned}
